SmartContracts/ModellingOfBugs/DeusFinacePriceOracleManipulation/voting.dfy
@@ -38,12 +38,12 @@ class Vote {
   {
     proposal := Proposal(block.timestamp, msg.sender);
   }
-  method vote(amount : uint, msg:Msg)
+  method vote(amount : uint256, msg:Msg)
     requires proposal.sTime as nat + 2  > block.timestamp as nat
-    requires (if msg.sender in votingToken then votingToken[msg.sender] else 0) as nat + amount as nat < MAX_UINT256
+    requires msg.sender !in votingToken ||  votingToken[msg.sender] as nat + amount as nat <= MAX_UINT256
     modifies this
   {
-
+    mapAddVoting(votingToken, msg.sender, amount as nat);
     votingToken := votingToken[msg.sender :=(if msg.sender in votingToken then votingToken[msg.sender] else 0) + amount]; // transfer from sender to this contract using token's method.
     totalamount := totalamount + amount as nat;
   }
@@ -52,11 +52,11 @@ class Vote {
     modifies this
     requires proposal.sTime != 0
     requires proposal.sTime as nat + 2  < block.timestamp as nat
+    ensures sum(votingToken) == totalamount
     //  requires sum(votingToken) == totalamount as nat
   {
     //  require(votingToken.balanceOf(address(this))*2 >
     //  votingToken.totalSupply(), "vote failed");
-    assert(sum(votingToken) == totalamount);
     owner := proposal.newOwner;
   }
   constructor(msg: Msg)
@@ -67,3 +67,9 @@ class Vote {
   }
 }
 
+
+lemma mapAddVoting(m: map<Address, uint256>, k: Address, v: nat)
+  requires (if k in m then m[k] else 0) as nat + v <= MAX_UINT256
+  //  m ++ [k, v] is m with the value at k incremented by v (0 is not in key)
+  //  sum(m ++ [k,v]) == sum(m) + v
+  ensures sum(m[k := ((if k in m then m[k] else 0) as nat + v) as uint256]) >= sum(m) + v
